tests/fstar/hashmap_on_disk/HashmapMain.Properties.fst
@@ -19,7 +19,7 @@ val state_v : state -> hashmap_hash_map_t u64
 assume
 val serialize_lem (hm : hashmap_hash_map_t u64) (st : state) : Lemma (
   match hashmap_utils_serialize_fwd hm st with
-  | Fail -> True
+  | Fail _ -> True
   | Return (st', ()) -> state_v st' == hm)
   [SMTPat (hashmap_utils_serialize_fwd hm st)]
 
@@ -27,7 +27,7 @@ val serialize_lem (hm : hashmap_hash_map_t u64) (st : state) : Lemma (
 assume
 val deserialize_lem (st : state) : Lemma (
   match hashmap_utils_deserialize_fwd st with
-  | Fail -> True
+  | Fail _ -> True
   | Return (st', hm) -> hm == state_v st /\ st' == st)
   [SMTPat (hashmap_utils_deserialize_fwd st)]
 
@@ -38,11 +38,11 @@ val deserialize_lem (st : state) : Lemma (
 /// in the hash map previously stored on disk.
 val insert_on_disk_fwd_lem (key : usize) (value : u64) (st : state) : Lemma (
   match insert_on_disk_fwd key value st with
-  | Fail -> True
+  | Fail _ -> True
   | Return (st', ()) ->
     let hm = state_v st in
     match hashmap_hash_map_insert_fwd_back u64 hm key value with
-    | Fail -> False
+    | Fail _ -> False
     | Return hm' -> hm' == state_v st')
 
 let insert_on_disk_fwd_lem key value st = ()
