tests/fstar/misc/Paper.fst
@@ -7,13 +7,13 @@ open Primitives
 
 (** [paper::ref_incr] *)
 let ref_incr_fwd_back (x : i32) : result i32 =
-  begin match i32_add x 1 with | Fail -> Fail | Return x0 -> Return x0 end
+  begin match i32_add x 1 with | Fail e -> Fail e | Return x0 -> Return x0 end
 
 (** [paper::test_incr] *)
 let test_incr_fwd : result unit =
   begin match ref_incr_fwd_back 0 with
-  | Fail -> Fail
-  | Return x -> if not (x = 1) then Fail else Return ()
+  | Fail e -> Fail e
+  | Return x -> if not (x = 1) then Fail Failure else Return ()
   end
 
 (** Unit test for [paper::test_incr] *)
@@ -31,18 +31,20 @@ let choose_back
 (** [paper::test_choose] *)
 let test_choose_fwd : result unit =
   begin match choose_fwd i32 true 0 0 with
-  | Fail -> Fail
+  | Fail e -> Fail e
   | Return z ->
     begin match i32_add z 1 with
-    | Fail -> Fail
+    | Fail e -> Fail e
     | Return z0 ->
       if not (z0 = 1)
-      then Fail
+      then Fail Failure
       else
         begin match choose_back i32 true 0 0 z0 with
-        | Fail -> Fail
+        | Fail e -> Fail e
         | Return (x, y) ->
-          if not (x = 1) then Fail else if not (y = 0) then Fail else Return ()
+          if not (x = 1)
+          then Fail Failure
+          else if not (y = 0) then Fail Failure else Return ()
         end
     end
   end
@@ -63,14 +65,14 @@ let rec list_nth_mut_fwd (t : Type0) (l : list_t t) (i : u32) : result t =
     then Return x
     else
       begin match u32_sub i 1 with
-      | Fail -> Fail
+      | Fail e -> Fail e
       | Return i0 ->
         begin match list_nth_mut_fwd t tl i0 with
-        | Fail -> Fail
+        | Fail e -> Fail e
         | Return x0 -> Return x0
         end
       end
-  | ListNil -> Fail
+  | ListNil -> Fail Failure
   end
 
 (** [paper::list_nth_mut] *)
@@ -82,14 +84,14 @@ let rec list_nth_mut_back
     then Return (ListCons ret tl)
     else
       begin match u32_sub i 1 with
-      | Fail -> Fail
+      | Fail e -> Fail e
       | Return i0 ->
         begin match list_nth_mut_back t tl i0 ret with
-        | Fail -> Fail
+        | Fail e -> Fail e
         | Return tl0 -> Return (ListCons x tl0)
         end
       end
-  | ListNil -> Fail
+  | ListNil -> Fail Failure
   end
 
 (** [paper::sum] *)
@@ -97,9 +99,12 @@ let rec sum_fwd (l : list_t i32) : result i32 =
   begin match l with
   | ListCons x tl ->
     begin match sum_fwd tl with
-    | Fail -> Fail
+    | Fail e -> Fail e
     | Return i ->
-      begin match i32_add x i with | Fail -> Fail | Return i0 -> Return i0 end
+      begin match i32_add x i with
+      | Fail e -> Fail e
+      | Return i0 -> Return i0
+      end
     end
   | ListNil -> Return 0
   end
@@ -110,17 +115,17 @@ let test_nth_fwd : result unit =
   let l0 = ListCons 3 l in
   let l1 = ListCons 2 l0 in
   begin match list_nth_mut_fwd i32 (ListCons 1 l1) 2 with
-  | Fail -> Fail
+  | Fail e -> Fail e
   | Return x ->
     begin match i32_add x 1 with
-    | Fail -> Fail
+    | Fail e -> Fail e
     | Return x0 ->
       begin match list_nth_mut_back i32 (ListCons 1 l1) 2 x0 with
-      | Fail -> Fail
+      | Fail e -> Fail e
       | Return l2 ->
         begin match sum_fwd l2 with
-        | Fail -> Fail
-        | Return i -> if not (i = 7) then Fail else Return ()
+        | Fail e -> Fail e
+        | Return i -> if not (i = 7) then Fail Failure else Return ()
         end
       end
     end
@@ -133,13 +138,13 @@ let _ = assert_norm (test_nth_fwd = Return ())
 let call_choose_fwd (p : (u32 & u32)) : result u32 =
   let (px, py) = p in
   begin match choose_fwd u32 true px py with
-  | Fail -> Fail
+  | Fail e -> Fail e
   | Return pz ->
     begin match u32_add pz 1 with
-    | Fail -> Fail
+    | Fail e -> Fail e
     | Return pz0 ->
       begin match choose_back u32 true px py pz0 with
-      | Fail -> Fail
+      | Fail e -> Fail e
       | Return (px0, _) -> Return px0
       end
     end
